### grammar
Implementing Stanford CS143 concepts  

Implemented LL(1) and LR(0) (and almost SLR(1))

Tested on `python 3.4`. `pip3 install -r requirements.txt`

```
>>> from grammar import Grammar
>>> G = Grammar.from_text("""
...             E → TA
...             A → +TA | ɛ 
...             T → FB
...             B → ∗FB | ɛ
...             F → (E) | a
...             """)
>>> G.stats()

STATS
Axiom: E
Terminals: (,),+,a,∗
Non-Terminals: A,B,E,F,T
Rules:
A → +TA | ɛ
B → ∗FB | ɛ
E → TA
F → (E) | a
T → FB

╒════╤═══════╤══════════╕
│    │ FNE   │ FOLLOW   │
╞════╪═══════╪══════════╡
│ A  │ +     │ $,)      │
├────┼───────┼──────────┤
│ B  │ ∗     │ $,),+    │
├────┼───────┼──────────┤
│ E  │ (,a   │ $,)      │
├────┼───────┼──────────┤
│ F  │ (,a   │ $,),+,∗  │
├────┼───────┼──────────┤
│ T  │ (,a   │ $,),+    │
╘════╧═══════╧══════════╛

Parsing table:

╒═════╤═════════╤═══════╤═════════╤════════╤═════════╤═══════╕
│     │ (       │ )     │ +       │ a      │ ∗       │ $     │
╞═════╪═════════╪═══════╪═════════╪════════╪═════════╪═══════╡
│ A   │         │ A → ɛ │ A → +TA │        │         │ A → ɛ │
├─────┼─────────┼───────┼─────────┼────────┼─────────┼───────┤
│ B   │         │ B → ɛ │ B → ɛ   │        │ B → ∗FB │ B → ɛ │
├─────┼─────────┼───────┼─────────┼────────┼─────────┼───────┤
│ E   │ E → TA  │       │         │ E → TA │         │       │
├─────┼─────────┼───────┼─────────┼────────┼─────────┼───────┤
│ F   │ F → (E) │       │         │ F → a  │         │       │
├─────┼─────────┼───────┼─────────┼────────┼─────────┼───────┤
│ T   │ T → FB  │       │         │ T → FB │         │       │
╘═════╧═════════╧═══════╧═════════╧════════╧═════════╧═══════╛


>>> G.parse("a+a∗a")

╒═══════════════╤═════════╤═══════════════╕
│   (top) stack │   parse │        action │
╞═══════════════╪═════════╪═══════════════╡
│            E$ │  a+a∗a$ │  apply E → TA │
├───────────────┼─────────┼───────────────┤
│           TA$ │  a+a∗a$ │  apply T → FB │
├───────────────┼─────────┼───────────────┤
│          FBA$ │  a+a∗a$ │   apply F → a │
├───────────────┼─────────┼───────────────┤
│          aBA$ │  a+a∗a$ │         match │
├───────────────┼─────────┼───────────────┤
│           BA$ │   +a∗a$ │   apply B → ɛ │
├───────────────┼─────────┼───────────────┤
│            A$ │   +a∗a$ │ apply A → +TA │
├───────────────┼─────────┼───────────────┤
│          +TA$ │   +a∗a$ │         match │
├───────────────┼─────────┼───────────────┤
│           TA$ │    a∗a$ │  apply T → FB │
├───────────────┼─────────┼───────────────┤
│          FBA$ │    a∗a$ │   apply F → a │
├───────────────┼─────────┼───────────────┤
│          aBA$ │    a∗a$ │         match │
├───────────────┼─────────┼───────────────┤
│           BA$ │     ∗a$ │ apply B → ∗FB │
├───────────────┼─────────┼───────────────┤
│         ∗FBA$ │     ∗a$ │         match │
├───────────────┼─────────┼───────────────┤
│          FBA$ │      a$ │   apply F → a │
├───────────────┼─────────┼───────────────┤
│          aBA$ │      a$ │         match │
├───────────────┼─────────┼───────────────┤
│           BA$ │       $ │   apply B → ɛ │
├───────────────┼─────────┼───────────────┤
│            A$ │       $ │   apply A → ɛ │
├───────────────┼─────────┼───────────────┤
│             $ │       $ │        accept │
╘═══════════════╧═════════╧═══════════════╛

```
